---
title: Proof that H and I-H are Idempotent
author: 'Randi '
date: '2021-11-23'
slug: proof-that-h-and-i-h-are-idempotent
categories:
  - proof
tags:
  - proof writing
  - proof
  - multiple linear regression
  - X(X^TX)^-1X^T
  - yhat
  - I-H
  - abstratct math
  - statistics
  - hat matrix
  - idempotent
---

# Prove H and I-H are Idempotent 

Define the hat matrix $H=X(X^TX)^{-1}X^T$. 

For H to be Idempotent then $HH=H$

\begin{equation}\label{HH=H}
\begin{split}
HH & =[X(X^TX)^{-1}X^T][X(X^TX)^{-1}X^T]\\
& = X(X^TX)^{-1}X^TX(X^TX)^{-1}X^T\quad\quad(X^TX)^{-1}X^TX=1\\
& = X(X^TX)^{-1}X^T\\
& = H
\end{split}
\end{equation}

Therefore by the series of equalities H is idempotent. 

For I-H to be idempotent then $(I-H)(I-H)=I-H$

\begin{equation}\label{I-H}
\begin{split}
(I-H)(I-H) & =II-HI-IH+HH\quad\quad II=I, HI=IH=H, HH=H\\
& = I-H-H+H\\
& = I-H
\end{split}
\end{equation}

Therefor by the series of equalities I-H is idempotent. 

QED. 

